---
title: "Expectation Maximization"
layout: post
date: 2018-02-10 22:00
headerImage: false
tag:
- optimization
- expectation-maximization
category: blog
hidden: false
author: zhiyzuo
description: brief introduction to Expectation Maximization (EM) algorithm
---

___Last updated on 02-15-2018.___

___Table of Contents___
* Do not remove this line (it will not be displayed)
{:toc}

***

Note: All the materials below are based on the excellent lecture videos by Prof. Andrew Ng, along with the [lecture notes](http://cs229.stanford.edu/notes/cs229-notes8.pdf).

<iframe width="560" height="315" align="middle" src="https://www.youtube.com/embed/ZZGTuAkF-Hw" frameborder="0" allow="autoplay; encrypted-media" allowfullscreen></iframe>

<div class="breaker"></div>


```python
import numpy as np
import scipy as sp
```


```python
import seaborn as sns
from matplotlib import pyplot as plt
%matplotlib inline
```

<div class="breaker"></div>

### Introduction: Density estimation

We start by defining a problem in the context of unsupervised learning. Suppose we have 1 dimensional data, denoted by $\mathbf{x} = (x^{(1)}, ..., x^{(m)})$, shown as below.


```python
N = 100
mu_arr = np.array([1, 10])
sigma_arr = np.array([1, 1])
x = np.append(np.random.normal(mu_arr[0], sigma_arr[0], N), 
              np.random.normal(mu_arr[1], sigma_arr[1], N))
x[:10]
```




    array([ 1.00612457,  2.06217951,  1.08963858,  2.97049835,  1.01856583,
           -0.12178341,  0.68514333,  0.4269212 ,  0.43700963, -0.21670371])




```python
fig, ax = plt.subplots(figsize=(12,3))
ax.scatter(x[:N], np.zeros(N), c='green', marker=2, s=150)
ax.scatter(x[N:], np.zeros(N), c='orange', marker='x', s=150)
ax.set_ylim([-1e-4, 1e-4])
_ = ax.set_yticks([])
sns.distplot(x[:N], color='green')
sns.distplot(x[N:], color='orange')
```


![png](/assets/images/Expectation-Maximization_files/Expectation-Maximization_10_1.png)


However, we may not know the real labels for each data point in reality. This, naturally, introduces a latent (a.k.a. hiddent/unobserved) variable called $\mathbf{z} = (z^{(1)}, ..., z^{(m)})$, which is multinomial: $z^{(i)}$ indicates which distribution a specific point $x^{(i)}$ belongs to. In the example above, $z^{(i)}$ actually follows a Bernoulli, since there are only two possible outcomes.

In this case, we have a model: $p(\mathbf{x},\mathbf{z}; \Theta)$, where only $\mathbf{x}$ is observed. Our goal is to maximize $L(\Theta)=\prod_{i}p(x^{(i)};\Theta)$. It is common to instead maximize the ___log likelihood___: $\ell(\Theta)=\sum_{i}ln~p(x^{(i)}; \Theta)$. This is also called the ___incompelte data log likelihood___ because we do not know the latent variable $\mathbf{z}$ that indicate each data point's memebrship (to density which a data point belongs).

To gain more insights on why this problem is diffcult, we decompose the log likelihood:
<div>\begin{align}
\ell(\Theta) & = \sum_{i}ln~p(x^{(i)}; \Theta) \\
& = \sum_{i} ln \sum_{z^{(i)}} p(x^{(i)}, z^{(i)}; \Theta)
\end{align}</div>

Note that there is summation over $z^{(i)}$ inside logarithm. Even if individual joint probability distributions are in the exponential families, the summation still makes the derivative intractable.

---

### Jensen Inequality

Before we talk about how EM algorithm can help us solve the intractability, we need to introduce Jensen inequality. This will be used later to construct a (tight) lower bound of the log likelihood.

Definition:

> Let function $f$ be a convex function (e.g., $f'' \geq 0$). Let $x$ be a random variable. Then we have $f(E[x]) \leq E[f(x)]$.
> 
> Further, $f$ is ___strictly convex___ if $f'' > 0$. In such case, $f(E[x]) = E[f(x)]$ i.f.f. $x=E[x]$
>
> On the other hand, $f$ is concave if $f'' \leq 0$, and we have $f(E[x]) \geq E[f(x)]$.

A useful example (that will be applied in EM algorithm) is $f(x) = ln~x$ is ___strictly concave___ for $x > 0$. Proof:
<div>\begin{align}
f''(x) = \frac{d~}{dx} f'(x) = \frac{d~\frac{1}{x}}{dx} = -\frac{1}{x^2} < 0
\end{align}</div>

Therefore, we have $ln~E[x] \geq E[ln~x]$

Let's go with a concrete example by plotting $f(x) = ln~x$


```python
x = np.linspace(.1, 5, 100)
y = np.log(x)
fig, ax = plt.subplots(figsize=(8,4))
ax.scatter(x, y, color='green', marker='+')
## 1 (p=0.5)
ax.vlines(x=1, ymin=-2.5, ymax=0, linestyle='--', color='green')
ax.hlines(y=0, xmin=-.1, xmax=1, linestyle='--', color='green')
ax.text(x=1.1, y=np.log(.7), s='$f(1)=0$',
        fontdict={'size': 13})
## 4 (p=0.5)
ax.vlines(x=4, ymin=-2.5, ymax=np.log(4), linestyle='--', color='green')
ax.hlines(y=np.log(4), xmin=-.1, xmax=4, linestyle='--', color='green')
ax.text(x=4.1, y=np.log(3.1), 
        s='$f(4)=%.2f$'%(np.log(4)),
        fontdict={'size': 13}
       )
ax.plot([1, 4], np.log([1, 4]), color='green', linestyle='dotted')
# E(x) = (1+4)/2 = 2.5
ax.vlines(x=2.5, ymin=-2.5, ymax=np.log(2.5), linestyle='--', color='green')
ax.hlines(y=np.log(2.5), xmin=-.1, xmax=2.5, linestyle='--', color='green')
```


![png](/assets/images/Expectation-Maximization_files/Expectation-Maximization_21_1.png)


--- 

### EM Algorithm Formalization

#### Derivation

Now we can formarlize the problem, starting from the log likelihood from Section 1:

<div>\begin{align}
\ell(\Theta) & = \sum_i ln~\sum_{z^{(i)}} p(x^{(i)}, z^{(i)}; \Theta) \\
& = \sum_i ln~\sum_{z^{(i)}} q_i(z^{(i)}) \frac{p(x^{(i)}, z^{(i)}; \Theta)}{q_i(z^{(i)})}
\end{align}</div>

where $q_i(z^{(i)})$ is any arbitrary probability distribution for $z^{(i)}$ and thus:$q_i(z^{(i)}) \geq 0; \sum_{z^{(i)}}~q_i(z^{(i)}) = 1$.

It is interesting (actually important) to note  that the summation inside the logarithm, $\sum_{z^{(i)}} q_i(z^{(i)}) \frac{p(x^{(i)}, z^{(i)}; \Theta)}{q_i(z^{(i)})}$, takes the form of expectation of $\frac{p(x^{(i)}, z^{(i)}; \Theta)}{q_i(z^{(i)})}$, given $x^{(i)}$. Recall that $E[f(x)] = \sum_i p(x^{(i)})f(x^{(i)})$, where $p(x)$ is the probability mass function for $x^{(i)}$. Therefore, we can write the above into: 
<div>\begin{equation}
\ell(\Theta) = \sum_i ln~\sum_{z^{(i)}} E_{z^{(i)} \sim q_i(z^{(i)})}\Big[ \frac{p(x^{(i)}, z^{(i)}; \Theta)}{q_i(z^{(i)})} \Big]
\end{equation}</div>

Now, it is not difficult to see that we can apply Jensen Inequality on the term within the summation over $i$:

<div>
\begin{align}
\ell(\Theta) & = \sum_i ln~\sum_{z^{(i)}} E_{z^{(i)} \sim q_i(z^{(i)})}\Big[ \frac{p(x^{(i)}, z^{(i)}; \Theta)}{q_i(z^{(i)})} \Big] \\
& \geq \sum_i E_{z^{(i)} \sim q_i(z^{(i)})} \Big[ ln~\frac{p(x^{(i)}, z^{(i)}; \Theta)}{q_i(z^{(i)})} \Big] \\
& = \sum_i \sum_{z^{(i)}} q_i(z^{(i)})ln~\frac{p(x^{(i)}, z^{(i)}; \Theta)}{q_i(z^{(i)})}
\end{align}
</div>

In this way, we successfully construct the lower bound for $\ell(\Theta)$. However, this is not enough. Note that we want to squeeze the lower bound as much as we can to obtain the ___equality___. Based on Section 2, we need 

$$\frac{p(x^{(i)}, z^{(i)}; \Theta)}{q_i(z^{(i)})} = c$$

where $c$ is some constant. And this leads to

$$q_i(z^{(i)}) \propto p(x^{(i)}, z^{(i)}; \Theta)~~ s.t. \sum_{z^{(i)}} q_i(z^{(i)}) = 1$$

From the formula above, we can determine the choice of $q$

<div>
\begin{align}
q_i(z^{(i)}) & = \frac{p(x^{(i)}, z^{(i)}; \Theta)}{\sum_z p(x^{(i)}, z; \Theta)} \\
& = \frac{p(x^{(i)}, z^{(i)}; \Theta)}{p(x^{(i)}; \Theta)} \\
& = p(z^{(i)}\vert x^{(i)}; \Theta)
\end{align}
</div>

The last term is actually the posterior distribution of $z^{(i)}$ (soft membership) given the observation $x^{(i)}$ and the paramter $\Theta$


#### Algorithm Operationalization

EM is an iterative algorithm that consists of two steps:

- E step: Let $q_i(z^{(i)}) = p(z^{(i)}\vert x^{(i)}; \Theta)$. The gives a tight lower bound for $\ell(\Theta)$. This is actually maximizing the expectation shown above.
- M step: Update parameters to maximize the lower bound $\Theta := argmax_{\Theta} \sum_i \sum_{z^{(i)}} q_i(z^{(i)})ln~\frac{p(x^{(i)}, z^{(i)}; \Theta)}{q_i(z^{(i)})}$


#### Convergence

To prove the convergence of EM algorithm, we can prove the fact that $\ell(\Theta^{(t+1)}) \geq \ell(\Theta^{(t)})$ for any $t$, where $\Theta^{(t)}$ is the parameter estimatations at iteration $t$.

Recall that we choose $q_i(z^{(i)}) = p(z^{(i)}\vert x^{(i)}; \Theta)$ so that Jensen inequality will become ___equality___ such that:

<div> $$\ell(\Theta^{(t)})= \sum_i \sum_{z^{(i)}} q_i^{(t)}(z^{(i)})ln~\frac{p(x^{(i)}, z^{(i)}; \Theta^{(t)})}{q_i^{(t)}(z^{(i)})}$$ </div> 

In the M step, we then update our parameter to be $\Theta^{(t+1)}$ that maximizes the R.H.S. of the equation above:

<div>\begin{align}
\ell(\Theta^{(t+1)}) & = \sum_i \sum_{z^{(i)}} q_i^{(t+1)}(z^{(i)})ln~\frac{p(x^{(i)}, z^{(i)}; \Theta^{(t+1)})}{q_i^{(t+1)}(z^{(i)})} \\
& \geq \sum_i \sum_{z^{(i)}} q_i^{(t)}(z^{(i)})ln~\frac{p(x^{(i)}, z^{(i)}; \Theta^{(t+1)})}{q_i^{(t)}(z^{(i)})} \\
& \geq \sum_i \sum_{z^{(i)}} q_i^{(t)}(z^{(i)})ln~\frac{p(x^{(i)}, z^{(i)}; \Theta^{(t)})}{q_i^{(t)}(z^{(i)})} \\
& = \ell(\Theta^{(t)})
\end{align}</div>

Therefore, EM algorithm will make the log likelihood change monotonically. A common practice to monitor the convergence is to test if the difference of log likelihoods at two success iterations is less than some predefined tolerance parameter.

---

### Towards deeper understanding of EM: Evidence Lower Bound (ELBO)

We just derived the formulation of EM algorithm in details. However, one thing we did not do is to explicitly write out the decomposition of $\ell(\Theta)$. In fact, we can mathematically write out the log likelihood into the sum of two terms:
- $KL(q\vert \vert p) = \sum_{z} q(z) ln~ \frac{q(z)}{p(z \vert \mathbf{x}; \Theta)}$
- $\mathcal{L}(\mathbf{x}; \Theta) = \sum_{z} q(z)  ln~ \frac{p(\mathbf{x}, z; \Theta)}{q(z)}$

#### Derivation

<div>\begin{align}
ln~p(\mathbf{x}; \Theta) & = \sum_{z} q(z) ln p(\mathbf{x}; \Theta) \\
& [\text{Recall that } \sum_z q(z) = 1] \\
& = \sum_{z} q(z)  ln~ \frac{p(\mathbf{x}, z; \Theta)}{p(z \vert \mathbf{x}; \Theta)} \\
& = \sum_{z} q(z)  ln~ \frac{p(\mathbf{x}, z; \Theta)~q(z)}{p(z \vert \mathbf{x}; \Theta) ~q(z)} \\
& = \sum_{z} q(z)  ln~ \frac{p(\mathbf{x}, z; \Theta)}{q(z)}  + \sum_{z} q(z) ln~ \frac{q(z)}{p(z \vert \mathbf{x}; \Theta)}\\
& = \mathcal{L}(\mathbf{x}; \Theta) + KL(q\vert \vert p)
\end{align}</div>

#### ELBO

Here, we define evidence lower bound to be $ELBO = \mathcal{L}(\mathbf{x}; \Theta)$, because KL-divergence is non-negative. Specifically, the equality only holds when $q(z) = p(z \vert \mathbf{x}; \Theta)$. Therefore, $ELBO$ can be seen as a ___tight___ lower bound of the evidence (incomplete data likelihood):

$$ln~p(\mathbf{x}; \Theta) \geq ELBO$$

Such result is actually consistent with the previous derivation where we directly apply Jensen's inequality.

---

### Applying EM on Gaussian Mixtures

In this section, we will use an example of Gaussian Mixture to demonstrate the application of EM algorithm.

Suppose we have some data $\mathbf{x}=\{x^{(1)}, ..., x^{(m)}\}$, which some from $K$ different Gaussian distributions ($K$ mixtures). We will use the following notations:

- $\mu_k$: the mean of the $k^{th}$ Gaussian component
- $\Sigma_k$: the covariance matrix of the $k^{th}$ Gaussian component
- $\phi_k$: the multinomial parameter of a specific datapoint belonging to the $k^{th}$ componenet.
- $z^{(i)}$: the latent variable (multinomial) for each $x^{(i)}$

We also assume that the dimension of each $x^{(i)}$ is $n$.

The goal is: $max_{\mu, \Sigma, \phi}~ln~p(\mathbf{x};\mu, \Sigma, \phi)$. Therefore this follows exactly the EM framework.

#### E step

We set $w_j^{(i)} = q_i(z^{(i)}=j) = p(z^{(i)}=j \vert x^{(i)}; \mu, \Sigma, \phi)$.

#### M step

We will write down the lower bound and get derivatives for each of the three parameters.

<div>\begin{align} 
\sum_{i}^{m} \sum_{j}^{K} & q_i(z^{(i)}=j) ln~\frac{p(x^{(i)}, z^{(i)}=j; \mu, \Sigma, \phi)}{q_i(z^{(i)}=j)}  \\
&= \sum_{i}^{m} \sum_{j}^{K} q_i(z^{(i)}=j) ln~\frac{p(x^{(i)}\vert z^{(i)}=j; \mu, \Sigma) p(z^{(i)}=j; \phi)}{q_i(z^{(i)}=j)}
\end{align}</div>

Note that:
- $x^{(i)} \vert z^{(i)}=j; \mu, \Sigma \sim \mathcal{N}(\mu_j, \Sigma_j)$
- $z^{(i)}=j; \phi \sim Multi(\phi)$

We can then leverage these probability distributions and continue

<div>\begin{align}
ll := \sum_{i}^{m} \sum_{j}^{K} w_j^{(i)} ln~\frac{\frac{1}{\sqrt{(2\pi)^{n}\vert\Sigma_j\vert}}~exp\Big(-\frac{1}{2}(x^{(i)}-\mu_j)^{T}\Sigma_j^{-1}(x^{(i)}-\mu_j)\Big)~\phi_j}{w_j^{(i)}}
\end{align}</div>

Now, we need to maximize this lower bound for each of the three parameters. Many of the derivative on vector/matrix are based on [Matrix Cookbook](http://www.math.uwaterloo.ca/~hwolkowi//matrixcookbook.pdf)

##### Derivative of $\mu_j$

<div>\begin{align}
\nabla_{\mu_j} ll & = \nabla_{\mu_j} \sum_{i}^{m} w_j^{(i)} ln~\frac{\frac{1}{\sqrt{(2\pi)^{n}\vert\Sigma_j\vert}}~exp\Big(-\frac{1}{2}(x^{(i)}-\mu_j)^{T}\Sigma_j^{-1}(x^{(i)}-\mu_j)\Big)~\phi_j}{w_j^{(i)}} \\
& = \nabla_{\mu_j} \sum_{i}^{m} w_j^{(i)} \Big[ ln~\frac{\frac{1}{\sqrt{(2\pi)^{n}\vert\Sigma_j\vert}}~\phi_j}{w_j^{(i)}} + ln~exp\Big(-\frac{1}{2}(x^{(i)}-\mu_j)^{T}\Sigma_j^{-1}(x^{(i)}-\mu_j)\Big) \Big] \\
& = \nabla_{\mu_j} \sum_{i}^{m} w_j^{(i)} \Big[ \frac{1}{2}(x^{(i)}-\mu_j)^{T}\Sigma_j^{-1}(x^{(i)}-\mu_j) \Big] \\
& = -\frac{1}{2} \sum_{i}^{m} w_j^{(i)}  \nabla_{\mu_j}\Big[ (x^{(i)}-\mu_j)^{T}\Sigma_j^{-1}(x^{(i)}-\mu_j) \Big] \\
& \big[ \text{For } f(x) = x^T A x \text{: } \nabla_{x} f(x) = (A+A^T)x\big] \\
& = \frac{1}{2} \sum_{i}^{m} w_j^{(i)}  \nabla_{(x^{i} - \mu_j)}\Big[ (x^{(i)}-\mu_j)^{T}\Sigma_j^{-1}(x^{(i)}-\mu_j) \Big] \\
& = \frac{1}{2} \sum_{i}^{m} w_j^{(i)}  \Big[ (\Sigma_j^{-1} + (\Sigma_j^{-1})^T) (x^{(i)} - \mu_j) \Big] \\
& \big[ \text{Note that } \Sigma_j \text{ is symmetric so we have } (\Sigma_j^{-1})^T = (\Sigma_j^{T})^{-1} =\Sigma_j^{-1} \big] \\
& = \sum_{i}^{m} w_j^{(i)}  \Big[ \Sigma_j^{-1} (x^{(i)} - \mu_j) \Big] \\
\end{align}</div>

Set the last term zero, we have

<div>\begin{align}
\nabla_{\mu_j} ll & = 0 \\
\sum_{i}^{m} w_j^{(i)}  \Big[ \Sigma_j^{-1} (x^{(i)} - \mu_j) \Big] & = 0  \\
\sum_{i}^{m} w_j^{(i)}(x^{(i)} - \mu_j) & = 0 \\
\sum_{i}^{m} w_j^{(i)} x^{(i)} & = \sum_{i}^{m} w_j^{(i)} \mu_j \\
\mu_j & = \frac{\sum_{i}^{m} w_j^{(i)} x^{(i)}}{\sum_{i}^{m} w_j^{(i)}}
\end{align}</div>

##### Derivative of $\Sigma_j$

<div>\begin{align}
\nabla_{\Sigma_j} ll & = \nabla_{\Sigma_j} \sum_{i}^{m} w_j^{(i)} ln~\frac{\frac{1}{\sqrt{(2\pi)^{n}\vert\Sigma_j\vert}}~exp\Big(-\frac{1}{2}(x^{(i)}-\mu_j)^{T}\Sigma_j^{-1}(x^{(i)}-\mu_j)\Big)~\phi_j}{w_j^{(i)}} \\
& = \sum_{i}^{m} w_j^{(i)} \nabla_{\Sigma_j} \Big[ ln~\frac{1}{\sqrt{\vert\Sigma_j\vert}} - \frac{1}{2}(x^{(i)}-\mu_j)^{T}\Sigma_j^{-1}(x^{(i)}-\mu_j) \Big] \\
& = -\frac{1}{2} \sum_{i}^{m} w_j^{(i)} \Big[ \frac{\partial~ln~\vert\Sigma_j\vert}{\partial \Sigma_j} + \frac{\partial}{\partial \Sigma_j} (x^{(i)}-\mu_j)^{T}\Sigma_j^{-1}(x^{(i)}-\mu_j) \Big] \\
\end{align}</div>

First, we consider the derivative of the  first term in the square bracket:

<div>\begin{align}
\frac{\partial ln~\vert\Sigma_j\vert}{\partial \Sigma_j} & = \frac{1}{\vert\Sigma_j\vert} \frac{\partial \vert\Sigma_j\vert}{\partial \Sigma_j} \\
& = \frac{1}{\vert\Sigma_j\vert}\vert\Sigma_j\vert (\Sigma_j^{-1})^T \\
& = \Sigma_j^{-1}
\end{align}</div>

Then, we do the second term

<div>\begin{align}
\frac{\partial}{\partial \Sigma_j} (x^{(i)}-\mu_j)^{T}\Sigma_j^{-1}(x^{(i)}-\mu_j) & = -\Sigma_j^{-1}(x^{(i)}-\mu_j)(x^{(i)}-\mu_j)^{T} \Sigma_j^{-1} \\
\end{align}</div>

Combined these results back and set it to zero, we have:

<div>\begin{align}
\nabla_{\Sigma_j} ll & = -\frac{1}{2} \sum_i^{m} w_j^{(i)} \Big[ \Sigma_j^{-1} - \Sigma_j^{-1}(x^{(i)}-\mu_j)(x^{(i)}-\mu_j)^{T} \Sigma_j^{-1} \Big]\\
& = -\frac{1}{2} \sum_i^{m} w_j^{(i)} \Big[ I - \Sigma_j^{-1}(x^{(i)}-\mu_j)(x^{(i)}-\mu_j)^{T} \Big] \Sigma_j^{-1} \stackrel{set}{=} 0 \\
\end{align}</div>

Rearrange the equation and we have:

<div>\begin{align}
\sum_i^{m} w_j^{(i)} \Big[ \Sigma_j  - (x^{(i)}-\mu_j)(x^{(i)}-\mu_j)^{T} \Big] &= 0 \\
\sum_i^{m} w_j^{(i)} \Sigma_j &= \sum_i^{m} w_j^{(i)} (x^{(i)}-\mu_j)(x^{(i)}-\mu_j)^{T} \\
\Sigma_j & = \frac{\sum_i^{m} w_j^{(i)} (x^{(i)}-\mu_j)(x^{(i)}-\mu_j)^{T}}{\sum_i^{m} w_j^{(i)}}
\end{align}</div>

##### Derivative of $\phi_j$

This is relatively simpler but we need to apply Lagrange multipliers because $\sum_j \phi_j = 1$.

<div>\begin{align}
ll & = \sum_{i}^{m} \sum_{l}^{k} w_l^{(i)} ln~\frac{\frac{1}{\sqrt{(2\pi)^{n}\vert\Sigma_l\vert}}~exp\Big(-\frac{1}{2}(x^{(i)}-\mu_l)^{T}\Sigma_l^{-1}(x^{(i)}-\mu_l)\Big)~\phi_l}{w_l^{(i)}} \\
& =  \sum_{i}^{m} \sum_{l}^{k} w_l^{(i)} ln~\phi_l \\
\end{align}</div>

We need to construct Lagrangian, with $\lambda$ as the Lagrange multiplier:

$$\mathcal{L}(\phi) =  ll + \lambda (\sum_l^{k} \phi_l - 1)$$

We will take derivative on $\mathcal{L}$ and set it to zero:

<div>\begin{align}
\frac{\partial \mathcal{L}(\phi)}{\partial \phi_j} & = \frac{\partial}{\partial \phi_j} \Big[ ll + \lambda (\sum_l^{k} \phi_l - 1) \Big] \\
& = \sum_i w_j^{(i)} \frac{1}{\phi_j} + \lambda \stackrel{set}{=} 0\\
\end{align}</div>

Rearrange and we will have $\phi_j = -\frac{\sum_i w_j^{(i)}}{\lambda}$. Recall that $\sum_j \phi_j = 1$, we have:

<div>\begin{align}
\sum_j \phi_j & = \sum_j -\frac{\sum_i w_j^{(i)}}{\lambda} = 1\\
\lambda & = -\sum_j \sum_i w_j^{(i)} \\
& = -\sum_j \sum_i p(z^{(i)}=j\vert x^{(i)}) \\
& = -\sum_i 1 = -m
\end{align}</div>

Finally, we have:

$$\phi_j = \frac{\sum_i w_j^{(i)}}{m}$$

---

### Real example


```python
class GMM(object):
    def __init__(self, X, k=2):
        # dimension
        X = np.asarray(X)
        self.m, self.n = X.shape
        self.data = X.copy()
        # number of mixtures
        self.k = k
        
    def _init(self):
        # init mixture means/sigmas
        self.mean_arr = np.asmatrix(np.random.random((self.k, self.n)))
        self.sigma_arr = np.array([np.asmatrix(np.identity(self.n)) for i in range(self.k)])
        self.phi = np.ones(self.k)/self.k
        self.w = np.asmatrix(np.empty((self.m, self.k), dtype=float))
        #print(self.mean_arr)
        #print(self.sigma_arr)
    
    def fit(self, tol=1e-4):
        self._init()
        num_iters = 0
        ll = 1
        previous_ll = 0
        while(ll-previous_ll > tol):
            previous_ll = self.loglikelihood()
            self._fit()
            num_iters += 1
            ll = self.loglikelihood()
            print('Iteration %d: log-likelihood is %.6f'%(num_iters, ll))
        print('Terminate at %d-th iteration:log-likelihood is %.6f'%(num_iters, ll))
    
    def loglikelihood(self):
        ll = 0
        for i in range(self.m):
            tmp = 0
            for j in range(self.k):
                #print(self.sigma_arr[j])
                tmp += sp.stats.multivariate_normal.pdf(self.data[i, :], 
                                                        self.mean_arr[j, :].A1, 
                                                        self.sigma_arr[j, :]) *\
                       self.phi[j]
            ll += np.log(tmp) 
        return ll
    
    def _fit(self):
        self.e_step()
        self.m_step()
        
    def e_step(self):
        # calculate w_j^{(i)}
        for i in range(self.m):
            den = 0
            for j in range(self.k):
                num = sp.stats.multivariate_normal.pdf(self.data[i, :], 
                                                       self.mean_arr[j].A1, 
                                                       self.sigma_arr[j]) *\
                      self.phi[j]
                den += num
                self.w[i, j] = num
            self.w[i, :] /= den
            assert self.w[i, :].sum() - 1 < 1e-4
            
    def m_step(self):
        for j in range(self.k):
            const = self.w[:, j].sum()
            self.phi[j] = 1/self.m * const
            _mu_j = np.zeros(self.n)
            _sigma_j = np.zeros((self.n, self.n))
            for i in range(self.m):
                _mu_j += (self.data[i, :] * self.w[i, j])
                _sigma_j += self.w[i, j] * ((self.data[i, :] - self.mean_arr[j, :]).T * (self.data[i, :] - self.mean_arr[j, :]))
                #print((self.data[i, :] - self.mean_arr[j, :]).T * (self.data[i, :] - self.mean_arr[j, :]))
            self.mean_arr[j] = _mu_j / const
            self.sigma_arr[j] = _sigma_j / const
        #print(self.sigma_arr)
```

Setup dataset.


```python
X = np.random.multivariate_normal([0, 3], [[0.5, 0], [0, 0.8]], 20)
X = np.vstack((X, np.random.multivariate_normal([20, 10], np.identity(2), 50)))
X.shape
```




    (70, 2)




```python
gmm = GMM(X)
gmm.fit()
```

    Iteration 1: log-likelihood is -396.318688
    Iteration 2: log-likelihood is -358.902036
    Iteration 3: log-likelihood is -357.894632
    Iteration 4: log-likelihood is -353.797418
    Iteration 5: log-likelihood is -332.842685
    Iteration 6: log-likelihood is -287.787552
    Iteration 7: log-likelihood is -277.701280
    Iteration 8: log-likelihood is -268.521010
    Iteration 9: log-likelihood is -249.376342
    Iteration 10: log-likelihood is -230.906536
    Iteration 11: log-likelihood is -230.883025
    Iteration 12: log-likelihood is -230.883025
    Terminate at 12-th iteration:log-likelihood is -230.883025



```python
gmm.mean_arr
```




    matrix([[-0.05739539,  2.69216832],
            [20.04929409,  9.69219807]])




```python
gmm.sigma_arr
```




    array([[[0.30471149, 0.27830426],
            [0.27830426, 1.3309902 ]],
    
           [[0.94378014, 0.07495073],
            [0.07495073, 1.13089165]]])




```python
gmm.phi
```




    array([0.28571429, 0.71428571])


